IrisCore/EntailEnv.thy
@@ -1,5 +1,5 @@
 theory EntailEnv
-imports Misc
+imports Misc 
 begin
 
 subsubsection \<open>An environment for entailments\<close>
@@ -9,113 +9,149 @@ text \<open>
 \<close>
 
 declare [[typedef_overloaded = true]]
-datatype entail_env = Env (pure: "bool fset") (pers: "iprop list") (spatial: "iprop list")
+datatype entail_env = Env (pers: "iprop fset") (spatial: "iprop list") (* maybe multiset?*)
 
 instantiation entail_env :: plus begin
 definition plus_entail_env :: "entail_env \<Rightarrow> entail_env \<Rightarrow> entail_env" where
   "plus_entail_env e1 e2 = 
-    Env (pure e1 |\<union>| pure e2) (pers e1 @ pers e2) (spatial e1 @ spatial e2)"
+    Env (pers e1 |\<union>| pers e2) (spatial e1 @ spatial e2)"
 instance ..
 end
 
 definition env_iprop :: "entail_env \<Rightarrow> iprop" where
-  "env_iprop env = sep_fold_list (sep_fold_list ([\<^emph>\<^sub>m] upred_pure (pure env)) (pers env)) (spatial env)"
+  "env_iprop env = [\<^emph>\<^sub>l [\<^emph>\<^sub>m] id (pers env)] (spatial env)"
   
 lemma sep_list_singleton: "P \<equiv> [\<^emph>\<^sub>l] [P]" by (auto simp: upred_true_sep upred_sep_comm)
-
-lemma sep_list_ind: "P \<equiv> [\<^emph>\<^sub>l] P' \<Longrightarrow> P\<^emph>Q \<equiv> [\<^emph>\<^sub>l] (P'@[Q])"
-  by auto
-
-lemma sep_list_dual: "P\<^emph>Q \<equiv> [\<^emph>\<^sub>l Q] [P]"
-  by (auto simp: upred_sep_comm)
-
-lemma sep_list_step: "[\<^emph>\<^sub>l Q] ((P\<^emph>R)#Seps) \<equiv> [\<^emph>\<^sub>l Q] (P#R#Seps)"
-  by simp (smt (verit, ccfv_SIG) upred_sep_comm upred_sep_comm2_eq)
 
 lemma sep_list_acc:"[\<^emph>\<^sub>l P\<^emph>Q] Seps = P \<^emph> [\<^emph>\<^sub>l Q] Seps"
   by (induction Seps arbitrary: Q) (simp_all add: upred_sep_assoc_eq)
 
 lemma sep_list_cons: "[\<^emph>\<^sub>l P] (Q#Seps) = Q \<^emph> [\<^emph>\<^sub>l P] Seps"
-  by (metis (no_types, lifting) foldl_Cons  sep_list_acc upred_sep_comm)
-  
-lemma envI: "[\<^emph>\<^sub>l] P \<equiv> ([\<^emph>\<^sub>l] P) \<^emph> (env_iprop (Env {||} [] []))"
-  by (simp add: env_iprop_def sep_fold_fset_def 
-    comp_fun_commute.ffold_empty[OF sep_comp_fun_commute] upred_true_sep)
+  by (metis (no_types, lifting) foldl_Cons sep_list_acc upred_sep_comm)
 
-lemma pure_insert_idem: "b |\<in>| pure e \<Longrightarrow> env_iprop (Env (finsert b (pure e)) (pers e) (spatial e))
-  \<equiv> env_iprop e"
-  by (simp add: env_iprop_def sep_fold_fset_def finsert_absorb)
+lemma sep_list_step: "[\<^emph>\<^sub>l Q] ((P\<^emph>R)#Seps) \<equiv> [\<^emph>\<^sub>l Q] (P#R#Seps)"
+  by (smt (verit, del_insts) foldl_Nil foldl_append sep_list_cons upred_sep_assoc_eq)
 
-lemma move_pure_env: "([\<^emph>\<^sub>l] ((\<upharpoonleft>b)#P)) \<^emph> (env_iprop (Env pu pe sp)) \<equiv> 
-  ([\<^emph>\<^sub>l] P) \<^emph> (env_iprop (Env (finsert b pu) pe sp))" (is "?l \<equiv> ?r")
-proof -
-have "?l = ([\<^emph>\<^sub>l] P) \<^emph> \<upharpoonleft>b \<^emph> (env_iprop (Env pu pe sp))"
-  using sep_list_cons by (simp add: upred_sep_comm)
-then have "?l = ([\<^emph>\<^sub>l] P) \<^emph> \<upharpoonleft>b \<^emph> [\<^emph>\<^sub>l [\<^emph>\<^sub>l [\<^emph>\<^sub>m] upred_pure pu] pe] sp"
-  unfolding env_iprop_def by simp  
-then have "?l = ([\<^emph>\<^sub>l] P) \<^emph> (foldl (\<^emph>) (foldl (\<^emph>) (ffold (\<lambda>x a. a \<^emph> \<upharpoonleft>x) 
-  upred_emp pu) pe) sp) \<^emph> \<upharpoonleft>b"
-  apply (simp add: sep_fold_fset_def)
-  using upred_sep_assoc_eq upred_sep_comm2_eq by (smt (verit, del_insts))
-then have "?l = ([\<^emph>\<^sub>l] P) \<^emph> foldl (\<^emph>) (foldl (\<^emph>) (ffold (\<lambda>x a. a \<^emph> \<upharpoonleft>x) 
-  upred_emp pu) pe \<^emph> \<upharpoonleft>b) sp"
-  apply (simp add: sep_list_acc upred_sep_comm)
-  by (metis (no_types, lifting) upred_sep_assoc_eq upred_sep_comm)
-then have innermost_eq: "?l = ([\<^emph>\<^sub>l] P) \<^emph> foldl (\<^emph>) (foldl (\<^emph>) (ffold (\<lambda>x a. a \<^emph> \<upharpoonleft>x) 
-  upred_emp pu \<^emph> \<upharpoonleft>b) pe) sp"
-  by (simp add: sep_list_acc upred_sep_comm)
-have "?l = ?r" proof (cases "b |\<in>| pu")
-    case True
-    have "ffold (\<lambda>x a. a \<^emph> \<upharpoonleft>x) upred_emp pu \<^emph> (\<upharpoonleft>b) = 
-      ffold (\<lambda>x a. a \<^emph> \<upharpoonleft>x) upred_emp (pu |-| {|b|}) \<^emph> \<upharpoonleft>b \<^emph> \<upharpoonleft>b" (is "?l1 = _")
-      using comp_fun_commute.ffold_rec[OF sep_P_comp_fun_commute[of upred_pure] True] by metis
-    then have "?l1 = ffold (\<lambda>x a. a \<^emph> \<upharpoonleft>x) upred_emp (pu |-| {|b|}) \<^emph> \<upharpoonleft>b"
-      using pure_dupl by (smt (verit, ccfv_SIG) upred_sep_assoc_eq)
-    then have "?l1 = ffold (\<lambda>x a. a \<^emph> \<upharpoonleft>x) upred_emp pu" 
-      using comp_fun_commute.ffold_rec[OF sep_P_comp_fun_commute[of upred_pure] True] by metis
-    then have ff_pure_eq: "?l1 = ffold (\<lambda>x a. a \<^emph> \<upharpoonleft>x) upred_emp (finsert b pu)"
-      using finsert_absorb[OF True] by simp
-    show ?thesis unfolding innermost_eq
-    unfolding sep_fold_fset_def env_iprop_def
-    apply simp unfolding ff_pure_eq ..   
-  next
-    case False
-    show ?thesis unfolding innermost_eq 
-    unfolding env_iprop_def sep_fold_fset_def
-    unfolding comp_fun_commute.ffold_finsert[OF sep_P_comp_fun_commute[of upred_pure] False, symmetric]
-    by simp
-  qed
-then show "?l \<equiv> ?r" by simp
-qed
-   
-lemma move_pers_env: 
-  "([\<^emph>\<^sub>l] (Q#P)) \<^emph> (env_iprop (Env pu pe sp)) \<equiv> ([\<^emph>\<^sub>l] P) \<^emph> (env_iprop (Env pu (Q#pe) sp))"
-  unfolding sep_list_cons by (simp add: env_iprop_def sep_fold_fset_def)
-    (smt (verit) sep_list_acc upred_sep_comm upred_sep_comm2_eq)
+lemma sep_listI: "P \<equiv> P \<^emph> [\<^emph>\<^sub>l] []"
+  by (simp add: upred_true_sep)
+lemma sep_list_ind: "P \<^emph> Q \<^emph> [\<^emph>\<^sub>l] L \<equiv> P \<^emph> [\<^emph>\<^sub>l] (Q#L)"
+  using sep_list_cons sep_list_step by presburger
+lemma sep_list_drop: "P \<^emph> [\<^emph>\<^sub>l] L \<equiv> [\<^emph>\<^sub>l] (P#L)"
+  using sep_list_cons by auto
+
+lemma envI: "[\<^emph>\<^sub>l] P \<equiv> [\<^emph>\<^sub>l] P \<^emph> (env_iprop (Env {||} []))"
+  by (simp add: env_iprop_def sep_fold_fset_def comp_fun_commute.ffold_empty[OF sep_comp_fun_commute]
+    upred_true_sep)
+
+lemma sep_listE: "[\<^emph>\<^sub>l] [] \<^emph> env_iprop e \<equiv> env_iprop e"  
+  by (smt (verit) foldl_Nil upred_sep_comm upred_true_sep)
+
+lemma move_pure: "(b \<Longrightarrow> [\<^emph>\<^sub>l] Seps \<^emph> (env_iprop e) \<turnstile> Q) \<Longrightarrow> [\<^emph>\<^sub>l] (\<upharpoonleft>b)#Seps \<^emph> (env_iprop e) \<turnstile> Q"
+  by (metis (full_types) false_entails false_sep sep_list_cons upred_sep_comm upred_true_sep)
 
 lemma move_spatial_env: 
-  "([\<^emph>\<^sub>l] (Q#P)) \<^emph> (env_iprop (Env pu pe sp)) \<equiv> ([\<^emph>\<^sub>l] P) \<^emph> (env_iprop (Env pu pe (Q#sp)))"
+  "([\<^emph>\<^sub>l] (Q#P)) \<^emph> (env_iprop (Env pe sp)) \<equiv> ([\<^emph>\<^sub>l] P) \<^emph> (env_iprop (Env pe (Q#sp)))"
   unfolding sep_list_cons by (simp add: env_iprop_def sep_fold_fset_def)
     (smt (verit) sep_list_acc upred_sep_comm upred_sep_comm2_eq)
- 
+
+lemma move_pers_env: "persistent Q \<Longrightarrow>
+  env_iprop (Env pe (Q#sp)) \<turnstile> env_iprop (Env (finsert Q pe) sp)"
+  unfolding env_iprop_def sep_fold_fset_def
+  apply (cases "Q |\<in>| pe")
+  apply (simp_all add: finsert_absorb upred_frame upred_weakeningR sep_list_acc upred_sep_comm)
+  using comp_fun_commute.ffold_finsert[OF sep_P_comp_fun_commute[of id], simplified]
+  by (simp add: comp_fun_commute.ffold_finsert sep_comp_fun_commute sep_list_acc)
+
+lemma flip_spatial: "env_iprop (Env pe (Q#sp)) \<equiv> env_iprop (Env pe (sp@[Q]))"
+  by (simp add: sep_list_acc upred_sep_comm env_iprop_def)
+
+lemma env_exchange: 
+assumes "P\<^emph>Q\<turnstile>R" "persistent P" "P|\<in>|pe" "env_iprop (Env pe (R#sp))\<turnstile>T"
+shows "env_iprop (Env pe (Q#sp))\<turnstile>T"
+proof -
+  from assms(4) have "env_iprop (Env pe sp) \<^emph> R\<turnstile>T" 
+    by (simp add: sep_list_acc upred_sep_comm env_iprop_def sep_list_cons)  
+  from upred_entails_exchange[OF assms(1) this] have "env_iprop (Env pe sp) \<^emph> (P \<^emph> Q) \<turnstile> T" .
+  then have "env_iprop (Env pe sp) \<^emph> P \<^emph> Q \<turnstile> T" using upred_sep_assoc_eq by (metis (no_types, lifting))
+  with assms(3) have "env_iprop (Env (pe |-| {|P|}) sp) \<^emph> P \<^emph> P \<^emph> Q \<turnstile> T"
+    apply (simp add: env_iprop_def sep_fold_fset_def)
+    using comp_fun_commute.ffold_rec[OF sep_P_comp_fun_commute[of id] assms(3), simplified]
+    by (simp add: sep_list_acc upred_sep_comm)
+  then have "env_iprop (Env (pe |-| {|P|}) sp) \<^emph> Q \<^emph> (P \<^emph> P)  \<turnstile> T"
+    by (simp add: upred_sep_comm2L upred_sep_comm2_eq)
+  from upred_entails_exchange[OF upred_entail_eqR[OF persistent_dupl[OF assms(2)]] this]
+  have "env_iprop (Env (pe |-| {|P|}) sp) \<^emph> P \<^emph> Q \<turnstile> T"
+    by (simp add: upred_sep_comm2_eq)
+  then have "env_iprop (Env pe sp) \<^emph> Q \<turnstile> T" 
+    apply (simp add: env_iprop_def sep_fold_fset_def)
+    using comp_fun_commute.ffold_rec[OF sep_P_comp_fun_commute[of id] assms(3), simplified, symmetric]
+    by (metis (no_types, lifting) sep_list_acc upred_sep_comm)
+  then show ?thesis
+    by (simp add: env_iprop_def sep_fold_fset_def sep_list_acc upred_sep_comm)
+qed
+
+lemma do_proof_step_with_env:
+assumes "P\<turnstile>Q" "P = [\<^emph>\<^sub>l] P'" "\<forall>p \<in># (mset P'). (persistent p \<and> p |\<in>| pe) \<or> p \<in># (mset sp)" 
+  "Q = [\<^emph>\<^sub>l] Q'" "env_iprop (Env pe (Q'@sp)) \<turnstile> R"
+shows "env_iprop (Env pe sp) \<turnstile> R"
+sorry
+
 ML \<open>
   val sep_list_conv = Conv.rewr_conv @{thm sep_list_singleton}
     then_conv Conv.repeat_changed_conv (Conv.rewr_conv @{thm sep_list_step})
-  val list_env_conv = Conv.rewr_conv @{thm envI} then_conv Conv.repeat_changed_conv (
-    Conv.rewr_conv @{thm move_pure_env} else_conv (* Conv.rewr_conv @{thm move_pers_env} else_conv *) 
-    Conv.rewr_conv @{thm move_spatial_env})
-  fun params_conv ctxt cv ct = 
-    if Logic.is_all (Thm.term_of ct)
-    then Conv.arg_conv (Conv.abs_conv (fn (_, ctxt) => params_conv ctxt cv) ctxt) ct
-    else cv ct;
-  fun env_conv ctxt = sep_list_conv then_conv list_env_conv 
-    |> Conv.binop_conv 
+  fun embed_conv ctxt cv = (cv 
+    |> Conv.arg_conv (* Only transform the antecedent *)
+    |> Conv.fun_conv (* Go below the "\<turnstile>" *)
     |> HOLogic.Trueprop_conv
-    |> params_conv ctxt
-  fun sep_list_tac ctxt = CONVERSION (env_conv ctxt)
+    |> Conv.concl_conv ~1 (* Go below any assumptions *)
+    |> (fn cv => Conv.params_conv ~1 (K cv) ctxt))
+    handle CTERM _ => Conv.all_conv
+  fun env_conv ctxt = embed_conv ctxt (sep_list_conv then_conv Conv.rewr_conv @{thm envI})
+  fun move_to_env_conv ctxt = embed_conv ctxt (Conv.rewr_conv @{thm move_spatial_env})
+  fun drop_list_conv ctxt = embed_conv ctxt (Conv.rewr_conv @{thm sep_listE})
+  fun flip_spat_conv ctxt = embed_conv ctxt (Conv.rewr_conv @{thm flip_spatial})
+  
+  val reduce_list_conv_raw = Conv.rewr_conv @{thm sep_listI}
+    then_conv Conv.repeat_changed_conv (Conv.rewr_conv @{thm sep_list_ind})
+    then_conv (Conv.rewr_conv @{thm sep_list_drop})
+  fun reduce_list_conv ctxt = embed_conv ctxt reduce_list_conv_raw
 
-  val test = \<^cterm>\<open>\<And>x y z. (\<upharpoonleft>x) \<^emph> y \<^emph> z \<turnstile> y \<^emph> w \<^emph> (z::iprop)\<close>
-  val test_result = env_conv \<^context> test
+  fun sep_env_tac ctxt = FIRSTGOAL (
+    CONVERSION (env_conv ctxt) (* First introduce the list and emtpy env*)
+    THEN' (fn i => REPEAT_DETERM (CHANGED ((resolve_tac ctxt [@{thm move_pure}] ORELSE'
+      CONVERSION (move_to_env_conv ctxt)) i))) (* Then move all pure into context and rest into env*)
+    THEN' CONVERSION (drop_list_conv ctxt) (* Now drop the empty list *)
+  )
+
+  val persN = "pers_rules"
+  fun get_pers_thms lthy  = Proof_Context.get_thms lthy (Long_Name.qualify persN persN)
+  fun pers_tac ctxt = (fn i => (CHANGED (resolve_tac ctxt (get_pers_thms ctxt) i)))
+    |> REPEAT_ALL_NEW |> SOLVED'
+  fun strip_impl (Const (\<^const_name>\<open>Pure.imp\<close>,_) $ _ $ b) = strip_impl b
+    | strip_impl t = t
+  fun get_spatial_number thm = (if Thm.nprems_of thm > 0 then
+    Thm.cprem_of thm 1 |> Thm.term_of
+    |> strip_all_body
+    |> strip_impl
+    |> dest_comb |> snd (* Strip Trueprop*)
+    |> strip_comb |> snd |> hd (* Strip entails*)
+    |> dest_comb |> snd (* Strip env_iprop *)
+    |> dest_comb |> snd (*Strip Env Constructor *)
+    |> HOLogic.dest_list |> length
+    else 0) handle THM _ => 0 | CTERM _ => 0 | TERM _ => 0
+  fun is_pers_tac ctxt i thm = let val rounds = get_spatial_number thm in
+    REPEAT_DETERM_N rounds
+     ((resolve_tac ctxt @{thms upred_entails_trans[OF move_pers_env]} i
+       THEN HEADGOAL (pers_tac ctxt))
+     ORELSE ((CONVERSION (flip_spat_conv ctxt) THEN' simp_tac ctxt) i)) thm end
+
+  fun env_tac ctxt = sep_env_tac ctxt THEN (is_pers_tac ctxt 1)
 \<close>
 
+axiomatization w :: iprop
+lemma pers_w [pers_rule]: "persistent w" sorry
+
+lemma "\<And>x y z. (\<upharpoonleft>x) \<^emph> z \<^emph> w \<^emph> y \<turnstile> y \<^emph> w \<^emph> (z::iprop)"
+apply (tactic \<open>env_tac \<^context>\<close>)
+sorry
 end
