IrisCore/Invariant.thy
@@ -1,6 +1,6 @@
 theory Invariant
 imports DerivedConstructions BaseLogicShallow Frac AuthHeap Misc "../SpanningTree/SpanningTreeCameras"
-  Namespace iPropShallow EntailEnv
+  Namespace iPropShallow
 begin
 
 subsection \<open> Invariants \<close>
@@ -43,35 +43,43 @@ end
 
 lemma pcore_id_inv: "pcore_id_pred (constr_inv (map_view_frag \<iota> DfracDiscarded (Next (pre P)), \<epsilon>, \<epsilon>))"
   unfolding constr_inv_def prod_pcore_id_pred
-  apply (simp add: \<epsilon>_pcore_id_def del: \<epsilon>_option_def \<epsilon>_dfset_def \<epsilon>_dset_def)
-  by (rule pcore_id_frag[OF discarded_core_id])
+  by (simp add: \<epsilon>_pcore_id_def) (rule pcore_id_frag[OF discarded_core_id])
 
-lemma persistent_ownI: "persistent (ownI \<iota> P)"
+lemma persistent_ownI [pers_rule]: "persistent (ownI \<iota> P)"
   unfolding ownI_def own_inv_def by (rule persistent_core_own2[OF pcore_id_inv])
 
-lemma persistent_inv: "persistent (inv N P)"
+lemma persistent_inv [pers_rule]: "persistent (inv N P)"
   unfolding inv_def
   apply (rule persistent_exists)
   apply (rule persistent_conj)
   apply (rule persistent_pure)
   by (rule persistent_ownI)
 
+lemma constr_inv_valid: "\<lbrakk>valid mv; valid e; valid d\<rbrakk> \<Longrightarrow> valid (constr_inv (mv,e,d))"
+  unfolding constr_inv_def by (auto simp: prod_valid_def \<epsilon>_valid)
+
 lemma ownE_singleton_twice: "ownE (DSet {i}) \<^emph> ownE (DSet {i}) \<turnstile> \<upharpoonleft>False"
   unfolding ownE_def own_inv_def constr_inv_def
   apply (rule upred_entails_trans[OF upred_entail_eqR[OF own_op]])
   apply (rule upred_entails_trans[OF own_valid])
-  apply (simp add: op_prod_def \<epsilon>_left_id op_dset_def del: \<epsilon>_option_def \<epsilon>_dfset_def \<epsilon>_dset_def)
+  apply (simp add: op_prod_def \<epsilon>_left_id op_dset_def)
   apply transfer
-  by (simp add: prod_n_valid_def \<epsilon>_n_valid valid_raw_dset_def del: \<epsilon>_option_def \<epsilon>_dfset_def \<epsilon>_dset_def)
+  by (simp add: prod_n_valid_def \<epsilon>_n_valid valid_raw_dset_def)
+
+lemma ownD_singleton_twice: "ownD (DFSet {|i|}) \<^emph> ownD (DFSet {|i|}) \<turnstile> \<upharpoonleft>False"
+  unfolding ownD_def own_inv_def constr_inv_def
+  apply (auto simp: op_prod_def \<epsilon>_left_id op_dfset_def
+    intro!: upred_entails_trans[OF upred_entail_eqR[OF own_op]] upred_entails_trans[OF own_valid])
+  apply transfer
+  by (simp add: prod_n_valid_def \<epsilon>_n_valid valid_raw_dfset_def)
 
 lemma auth_map_both_validI: 
   "\<V>(constr_inv (map_view_auth (DfracOwn 1) m,\<epsilon>,\<epsilon>) \<cdot> constr_inv (map_view_frag k dq v,\<epsilon>,\<epsilon>)) \<turnstile>
     (fmlookup m k =\<^sub>u Some v) \<and>\<^sub>u \<upharpoonleft>(valid dq)"
 unfolding constr_inv_def op_prod_def
-apply (simp add: \<epsilon>_left_id auth_comb_opL del: \<epsilon>_dfset_def \<epsilon>_dset_def \<epsilon>_option_def split: prod.splits)
-apply (simp add: op_fun_def op_option_def del: \<epsilon>_dfset_def \<epsilon>_dset_def)
-apply transfer
-apply (simp add: prod_n_valid_def \<epsilon>_n_valid valid_raw_option_def del: \<epsilon>_dfset_def \<epsilon>_dset_def)
+apply (simp add: \<epsilon>_left_id auth_comb_opL split: prod.splits)
+apply transfer'
+apply (simp add: prod_n_valid_def \<epsilon>_n_valid valid_raw_option_def \<epsilon>_option_def)
 using map_view_both_valid by fastforce
 
 lemma invariant_lookup: 
@@ -87,19 +95,19 @@ lemma invariant_lookup:
   apply (metis dual_order.refl n_incl_def ofe_refl prod_cases3 total_n_inclI)
   by (metis \<epsilon>_left_id ofe_refl prod_cases3) 
 
-lemmas invariant_lookup' = persistent_keep[OF persistent_exists[OF persistent_sep[OF persistent_pure persistent_later[OF persistent_eq]]] invariant_lookup]
+lemma lookup_pers [pers_rule]: "persistent (\<exists>\<^sub>u Q. \<upharpoonleft>(fmlookup I \<iota> = Some Q) \<^emph> \<triangleright>(Q=\<^sub>uP))"
+  by pers_solver
 
 lemma ownI_open: "wsat \<^emph> ownI i P \<^emph> ownE (DSet {i}) \<turnstile> wsat \<^emph> (\<triangleright>P) \<^emph> ownD (DFSet {|i|})"
 unfolding wsat_def
 apply (rule pull_exists_antecedent2)
 apply (rule upred_existsE')
-apply (tactic \<open>sep_list_tac \<^context> 1\<close>)
-(* apply (rule upred_entails_trans[OF upred_entails_eq[OF upred_sep_comm]])
+apply (rule upred_entails_trans[OF upred_entails_eq[OF upred_sep_comm]])
 apply (rule upred_entails_trans[OF upred_sep_assoc])
 apply (rule upred_entails_trans[OF upred_sep_assoc'])
 apply (rule upred_entails_trans[OF upred_sep_comm3M])
 apply (rule upred_entails_trans[OF upred_sep_assoc_rev])
-apply (rule upred_entails_exchange[OF invariant_lookup'])
+apply (rule upred_entails_exchange[OF  persistent_keep[OF lookup_pers invariant_lookup]])
 apply (rule upred_entails_trans[OF upred_sep_assoc])
 apply (rule pull_exists_antecedentR)
 apply (rule upred_existsE')
@@ -110,7 +118,7 @@ apply (rule upred_pure_impl)
 apply (rule upred_entails_trans[OF upred_sep_assoc])
 apply (rule upred_entails_trans[OF upred_entails_eq[OF upred_sep_comm]])
 apply (rule upred_entails_trans[OF upred_sep_assoc])+
-apply (simp add: sep_map_dom_delete del: \<epsilon>_dfset_def \<epsilon>_dset_def)
+apply (simp add: sep_map_dom_delete)
 apply (rule upred_entails_trans[OF upred_sep_assoc])
 apply (rule upred_entails_trans[OF upred_sep_comm2R])
 apply (rule upred_disjE')
@@ -138,7 +146,7 @@ subgoal for I Q
   apply (rule upred_entails_trans[OF upred_sep_assoc])
   apply (rule upred_entails_trans[OF _ upred_entails_eq[OF upred_sep_comm]])
   apply (rule upred_frame)
-  apply (simp add: sep_map_dom_delete del: \<epsilon>_dfset_def \<epsilon>_dset_def)
+  apply (simp add: sep_map_dom_delete)
   apply (rule upred_entails_trans[OF upred_sep_assoc])+
   apply (rule upred_entails_trans[OF upred_sep_comm2R])
   apply (rule upred_frame)
@@ -149,8 +157,83 @@ apply (rule upred_entails_trans[OF upred_entails_eq[OF upred_sep_comm2L]])
 apply (rule upred_entails_trans[OF upred_sep_assoc'])
 apply (rule upred_entails_trans[OF upred_sep_assoc_rev])
 apply (rule upred_entails_exchange[OF ownE_singleton_twice])
-by simp *) sorry
- 
+by simp
+
+lemma ownI_close: "wsat \<^emph> ownI i P \<^emph> (\<triangleright> P) \<^emph> ownD (DFSet {|i|}) \<turnstile> wsat \<^emph> ownE (DSet {i})"
+apply (simp add: wsat_def)
+apply (auto simp: pull_exists_eq intro!: upred_existsE')
+apply (rule upred_entails_trans[OF upred_sep_comm3M])
+apply (rule upred_entails_trans[OF upred_sep_comm2R])
+apply (rule upred_entails_trans[OF upred_entails_eq[OF upred_sep_comm2L]])
+apply (auto simp: upred_sep_assoc_eq)
+apply (rule upred_entails_trans[OF upred_sep_comm4_2])
+apply (rule upred_entails_trans[OF upred_entails_eq[OF upred_sep_comm2L]])
+apply (auto simp: upred_sep_assoc_eq)
+apply (rule upred_entails_exchange[OF persistent_keep[OF lookup_pers invariant_lookup], unfolded upred_sep_assoc_eq])
+subgoal for I 
+apply (auto simp: upred_sep_assoc_eq intro!: upred_existsI[of _ _ I] pull_exists_antecedentR upred_existsE')
+apply (rule upred_entails_trans[OF upred_sep_comm2R])
+apply (auto simp: sep_map_dom_delete upred_sep_assoc_eq intro!: upred_pure_impl)
+apply (rule upred_entails_trans[OF upred_entails_eq[OF upred_sep_comm]])
+apply (simp add: upred_sep_assoc_eq)
+apply (rule upred_entails_trans[OF upred_sep_comm4_2])
+apply (rule upred_entails_trans[OF upred_sep_comm3M])
+apply (rule upred_entails_trans[OF upred_sep_comm2R])
+apply (auto simp: upred_sep_assoc_eq intro!: upred_disjE')
+subgoal for Q  
+  apply (rule upred_entails_trans[OF upred_sep_comm6_2R])
+  by (auto intro!: upred_entails_exchange[OF ownD_singleton_twice, unfolded upred_sep_assoc_eq])
+apply (auto simp: upred_sep_assoc_eq intro!: upred_frame)
+apply (rule upred_entails_trans[OF upred_entails_eq[OF upred_sep_comm2L]])
+apply (rule upred_entails_trans[OF upred_sep_comm2R])
+apply (auto simp: upred_sep_assoc_eq intro!: upred_frame)
+apply (rule upred_entails_trans[OF upred_entails_eq[OF upred_sep_comm2L]])
+apply (simp add: upred_sep_assoc_eq)
+apply (rule upred_entails_trans[OF upred_sep_comm4_2])
+apply (rule upred_entails_trans[OF upred_sep_comm3M])
+apply (rule upred_entails_trans[OF upred_sep_comm2R])
+apply (rule upred_entails_trans[OF _ upred_entails_eq[OF upred_sep_comm]])
+apply (auto simp: upred_sep_assoc_eq intro!: upred_frame upred_disjIL)
+apply (rule upred_entails_trans[OF upred_entails_eq[OF upred_sep_comm2L]])
+by (auto intro!: upred_entails_trans[OF upred_weakeningR2] 
+  upred_entails_trans[OF upred_entail_eqR[OF upred_later_sep]] upred_later_mono upred_eqE)
+done
+
+lemma ownI_alloc: "(\<forall>E::name dset. \<exists>i. \<not>i\<in>\<^sub>dE \<and> \<phi> i) \<Longrightarrow> 
+  (wsat \<^emph> \<triangleright> P) ==\<^emph> (\<exists>\<^sub>u i. \<upharpoonleft>(\<phi> i) \<^emph> wsat \<^emph> ownI i P)"
+apply (auto simp: wsat_def pull_exists_eq intro!: upred_wand_holdsI upred_existsE')
+apply (rule add_holds[OF own_unit,unfolded bupd_emp[OF upred_own_nothing_emp_eq]])
+apply (rule upred_entails_exchange[OF upred_wand_holdsE[OF own_updateP]])
+sorry (* Axiomatized as this requires too much low level ghost state reasoning for which I'd need to add
+    way more lemmata and things. *)
+
+lemma ownI_alloc_open: "(\<forall>E::name dset. \<exists>i. \<not>i\<in>\<^sub>dE \<and> \<phi> i) \<Longrightarrow> 
+  wsat ==\<^emph> (\<exists>\<^sub>u i. \<upharpoonleft>(\<phi> i) \<^emph> (ownE (DSet {i}) -\<^emph> wsat) \<^emph> ownI i P \<^emph> ownD (DFSet {|i|}))"
+apply (auto simp: wsat_def pull_exists_eq intro!: upred_wand_holdsI upred_existsE')
+sorry (* Axiomatized as this requires too much low level ghost state reasoning for which I'd need to add
+    way more lemmata and things. *)
+
+lemma wsat_alloc: "\<Rrightarrow>\<^sub>b (\<exists>\<^sub>u _::inv. wsat \<^emph> ownE (DSet UNIV))"
+apply (auto simp: upred_holds_entails)
+apply (rule add_own[of "constr_inv (map_view_auth (DfracOwn 1) fmempty,\<epsilon>,\<epsilon>)", 
+  OF constr_inv_valid[OF map_view_auth_valid \<epsilon>_valid \<epsilon>_valid]])
+apply (rule add_own[of "constr_inv (\<epsilon>,DSet UNIV,\<epsilon>)", 
+  OF constr_inv_valid[OF \<epsilon>_valid _ \<epsilon>_valid]])
+apply (simp add: valid_raw_dset_def valid_def)
+apply (rule add_own[of "constr_inv (\<epsilon>,\<epsilon>,DFSet {||})", 
+  OF constr_inv_valid[OF \<epsilon>_valid \<epsilon>_valid _], unfolded \<epsilon>_dfset_def[symmetric], OF \<epsilon>_valid])
+apply (auto simp: wsat_def pull_exists_eq own_inv_def ownE_def ownD_def 
+  intro!: upred_entails_trans[OF _ updI])
+apply (rule upred_existsI)
+apply (rule upred_existsI[of _ _ fmempty])
+apply (rule upred_entails_trans[OF upred_sep_comm2R])
+apply (auto intro!: upred_frame)
+apply (auto simp: lift_inv_fmap_def fmempty.rep_eq fmempty_def[symmetric] sep_fold_fset_def 
+  comp_fun_commute.ffold_empty[OF sep_P_comp_fun_commute]  intro!: upred_frame)
+apply (rule upred_entails_trans[OF upred_entails_eq[OF upred_sep_comm2L]])
+apply (rule upred_entails_trans[OF upred_sep_comm2R])
+by (auto simp: upred_weakeningL intro!: upred_frame)
+
 subsubsection \<open>Cancelable Invariants\<close>
 type_synonym cinvG = frac
 definition cinv_own :: "frac \<Rightarrow> iprop" where "cinv_own p = Own (constr_cinv (Some p))"
